cfrontend/Cshmgen.v
@@ -680,7 +680,7 @@ Definition transl_function (ce: composite_env) (f: Clight.function) : res functi
        (map fst (Clight.fn_temps f))
        tbody).
 
-Definition transl_fundef (ce: composite_env) (id: ident) (f: Clight.fundef) : res fundef :=
+Definition transl_fundef (ce: composite_env) (id: ident) (c: compartment) (f: Clight.fundef) : res fundef :=
   match f with
   | Internal g =>
       do tg <- transl_function ce g; OK(AST.Internal tg)
@@ -692,7 +692,7 @@ Definition transl_fundef (ce: composite_env) (id: ident) (f: Clight.fundef) : re
 
 (** ** Translation of programs *)
 
-Definition transl_globvar (id: ident) (ty: type) := OK tt.
+Definition transl_globvar (id: ident) (c: compartment) (ty: type) := OK tt.
 
 Definition transl_program (p: Clight.program) : res program :=
   transform_partial_program2 (transl_fundef p.(prog_comp_env)) transl_globvar p.
